Reversed the order of variables in the polynomials

bool/Algebra.v
@@ -12,7 +12,7 @@ Inductive null : poly -> Prop :=
 Inductive valid : nat -> poly -> Prop :=
 | valid_cst : forall k c, valid k (Cst c)
 | valid_poly : forall k p i q,
-  k <= i -> ~ null q -> valid (S i) p -> valid i q -> valid k (Poly p i q).
+  i < k -> ~ null q -> valid i p -> valid (S i) q -> valid k (Poly p i q).
 
 Hint Constructors valid.
 
@@ -64,8 +64,8 @@ Fixpoint valid_dec k p :=
 match p with
 | Cst c => true
 | Poly p i q =>
-  negb (decide (null q)) && decide (k <= i) &&
-    valid_dec (S i) p && valid_dec i q
+  negb (decide (null q)) && decide (i < k) &&
+    valid_dec i p && valid_dec (S i) q
 end.
 
 Instance Decidable_valid : forall n p, Decidable (valid n p) := {
@@ -76,7 +76,7 @@ abstract(revert n; induction p; simpl in *; intuition; bool; try_decide; auto).
 abstract(intros H; induction H; simpl in *; bool; try_decide; auto).
 Defined.
 
-Lemma valid_le_compat : forall k l p, valid k p -> l <= k -> valid l p.
+Lemma valid_le_compat : forall k l p, valid k p -> k <= l -> valid l p.
 Proof.
 intros k l p H Hl; induction H; constructor; eauto with arith.
 Qed.
@@ -129,7 +129,7 @@ intros p var1 var2 H; induction p; simpl; try_rewrite; auto.
 Qed.
 
 Lemma eval_suffix_compat : forall k p var1 var2,
-  (forall i, k <= i -> var1 i = var2 i) -> valid k p ->
+  (forall i, i < k -> var1 i = var2 i) -> valid k p ->
   eval var1 p = eval var2 p.
 Proof.
 intros k p var1 var2 Hvar Hv; revert var1 var2 Hvar.
@@ -163,8 +163,8 @@ match pl with
       (* Ensure validity *)
       if decide (null qs) then poly_add pl pr
       else Poly (poly_add pl pr) il qs
-    | Lt => Poly (poly_add pl (Poly pr ir qr)) il ql
-    | Gt => Poly (F pr) ir qr
+    | Gt => Poly (poly_add pl (Poly pr ir qr)) il ql
+    | Lt => Poly (F pr) ir qr
     end
   end
 end.
@@ -194,7 +194,7 @@ match p with
   if decide (null p) then p
   else Poly (Cst false) k p
 | Poly p i q =>
-  if decide (k <= i) then Poly (Cst false) k (Poly p i q)
+  if decide (i <= k) then Poly (Cst false) k (Poly p i q)
   else Poly (poly_mul_mon k p) i (poly_mul_mon k q)
 end.
 
@@ -268,31 +268,31 @@ Qed.
 
 Hint Extern 5 =>
 match goal with
-| [ |- min ?x ?y <= ?z ] =>
-  apply min_case_strong; intros; omega
-| [ |- ?z <= min ?x ?y ] =>
-  apply min_case_strong; intros; omega
+| [ |- max ?x ?y <= ?z ] =>
+  apply max_case_strong; intros; omega
+| [ |- ?z <= max ?x ?y ] =>
+  apply max_case_strong; intros; omega
 end.
-Hint Resolve le_min_r le_min_l.
+Hint Resolve le_max_r le_max_l.
 
 Lemma poly_add_valid_compat : forall kl kr pl pr, valid kl pl -> valid kr pr ->
-  valid (min kl kr) (poly_add pl pr).
+  valid (max kl kr) (poly_add pl pr).
 Proof.
 intros kl kr pl pr Hl Hr; revert kr pr Hr; induction Hl; intros kr pr Hr; simpl.
-  eapply valid_le_compat; [clear k|apply le_min_r].
+  eapply valid_le_compat; [clear k|apply le_max_r].
   now induction Hr; auto.
-  assert (Hle : min k kr <= min i kr).
-    apply min_case_strong; intros; apply min_case_strong; intros; auto; omega.
-  apply (valid_le_compat (min i kr)); auto.
+  assert (Hle : max (S i) kr <= max k kr).
+    apply max_case_strong; intros; apply max_case_strong; intros; auto; omega.
+  apply (valid_le_compat (max (S i) kr)); [|assumption].
   clear - IHHl1 IHHl2 Hl2 Hr H0; induction Hr.
     constructor; auto.
-      now rewrite <- (min_id (S i)); intuition.
+      now rewrite <- (max_id i); intuition.
     destruct (nat_compare_spec i i0); subst; try case_decide; repeat (constructor; intuition).
-        eapply valid_le_compat; eauto; instantiate; rewrite min_id; auto.
-        now eapply valid_le_compat; eauto; instantiate; rewrite min_id; auto.
-        now eapply valid_le_compat; eauto; instantiate; rewrite min_id; auto.
-        apply (valid_le_compat (min (S i) i0)); intuition.
-        apply (valid_le_compat (min i (S i0))); intuition.
+      now eapply valid_le_compat; eauto; instantiate; rewrite max_id; auto.
+      now eapply valid_le_compat; eauto; instantiate; rewrite max_id; auto.
+      now eapply valid_le_compat; eauto; instantiate; rewrite max_id; auto.
+      now apply (valid_le_compat (max (S i) i0)); intuition.
+      now apply (valid_le_compat (max i (S i0))); intuition.
 Qed.
 
 Lemma poly_opp_null_compat : forall p, null (poly_opp p) -> null p.
@@ -310,7 +310,7 @@ Lemma poly_mul_cst_valid_compat : forall k v p, valid k p -> valid k (poly_mul_c
 Proof.
 intros k v p H; induction H; simpl; [now auto|].
 case_decide; [|now auto].
-eapply (valid_le_compat (S i)); now auto.
+eapply (valid_le_compat i); [now auto|omega].
 Qed.
 
 Lemma poly_mul_mon_null_compat : forall i p, null (poly_mul_mon i p) -> null p.
@@ -318,30 +318,30 @@ Proof.
 intros i p; induction p; simpl; case_decide; simpl; inversion 1; intuition.
 Qed.
 
-Lemma poly_mul_mon_valid_compat : forall k i p, valid k p -> valid (min i k) (poly_mul_mon i p).
+Lemma poly_mul_mon_valid_compat : forall k i p, valid k p -> valid (max (S i) k) (poly_mul_mon i p).
 Proof.
-intros k i p H; induction H; simpl; case_decide; intuition.
-apply (valid_le_compat i); auto; constructor; intuition.
+intros k i p H; induction H; simpl poly_mul_mon; case_decide; intuition.
+apply (valid_le_compat (S i)); auto; constructor; intuition.
 match goal with [ H : null ?p |- _ ] => solve[inversion H] end.
 apply (valid_le_compat k); auto; constructor; intuition.
   assert (X := poly_mul_mon_null_compat); intuition eauto.
-  cutrewrite <- (min i (S i0) = S i0); intuition.
-  cutrewrite <- (min i i0 = i0); intuition.
+  now cutrewrite <- (max (S i) i0 = i0); intuition.
+  now cutrewrite <- (max (S i) (S i0) = S i0); intuition.
 Qed.
 
 Lemma poly_mul_valid_compat : forall kl kr pl pr, valid kl pl -> valid kr pr ->
-  valid (min kl kr) (poly_mul pl pr).
+  valid (max kl kr) (poly_mul pl pr).
 Proof.
 intros kl kr pl pr Hl Hr; revert kr pr Hr.
 induction Hl; intros kr pr Hr; simpl.
   apply poly_mul_cst_valid_compat; auto.
   apply (valid_le_compat kr); now auto.
-  apply (valid_le_compat (min (min (S i) kr) (min i (min i kr)))).
+  apply (valid_le_compat (max (max i kr) (max (S i) (max (S i) kr)))).
     case_decide.
-      apply (valid_le_compat (min (S i) kr)); now auto.
+      now apply (valid_le_compat (max i kr)); auto.
       apply poly_add_valid_compat; auto.
-      apply poly_mul_mon_valid_compat; intuition.
-    repeat apply min_case_strong; omega.
+      now apply poly_mul_mon_valid_compat; intuition.
+    repeat apply max_case_strong; omega.
 Qed.
 
 Section Eval.
@@ -351,7 +351,7 @@ Section Eval.
 Definition replace (var : nat -> bool) n z :=
   fun m => if decide (n = m) then z else var m.
 
-Lemma eval_replace_compat : forall k p var n z, valid k p -> n < k ->
+Lemma eval_replace_compat : forall k p var n z, valid k p -> k <= n ->
   eval (replace var n z) p = eval var p.
 Proof.
 intros k p var n z H Hlt; unfold replace.
