bool/Test.v
@@ -7,17 +7,24 @@ Goal forall a b c d e f g,
   (a && b && c && negb d && e && f && g) ||
   (a && b && c && d && negb e && f && g) ||
   (a && b && c && d && e && negb f && g) ||
-  (a && b && c && d && e && f && negb g) = true.
+  (a && b && c && d && e && f && negb g) ||
+  (a && b && c && d && e && f && g)
+  = true.
 Proof.
-intros; bool_simpl.
-
+Print BoolTactic.
+intros; bool_reify.
+ apply reduce_poly_of_formula_sound; vm_compute; reflexivity.
+Admitted.
 
 Goal forall a b c : bool, c || a = negb (b && negb b && (a || negb a)).
 Proof.
-intros; bool_simpl; unfold var_of_list; simpl.
-Print BoolTactic.
-Qed.
+intros; bool_ring.
+Admitted.
 
 Goal forall a b, (a || negb b) && (negb a || b) = true.
 intros; bool_ring.
 Admitted.
+
+Goal forall a b, (a || b || negb (a && b)) = true.
+Proof.
+intros; bool_ring.
